coq

coq/theories/dltt.v
@@ -8,115 +8,81 @@ Unset Printing Implicit Defensive.
 
 Module DLTT.
 
-Inductive elem T :=
-| Left  of T
-| Right of T
-| Null.
+Inductive sort : Type := U | L.
+
+Definition elem T := option (T * sort).
 
 Definition context T := seq (elem T).
-Definition cons_Left T (n : T) (Gamma : context T) : context T := 
-  Left n :: Gamma.
-Definition cons_Right T (n : T) (Gamma : context T) : context T := 
-  Right n :: Gamma.
-Definition cons_Null T (Gamma : context T) : context T := 
-  (Null _) :: Gamma.
+Definition cons_u T (n : T) (Gamma : context T) : context T := 
+  Some (n, U) :: Gamma.
+Definition cons_l T (n : T) (Gamma : context T) : context T := 
+  Some (n, L) :: Gamma.
+Definition cons_s T (n : T) (s : sort) (Gamma : context T) : context T := 
+  Some (n, s) :: Gamma.
+Definition cons_n T (Gamma : context T) : context T := 
+  None :: Gamma.
 
-Notation "m :L Gamma" := (cons_Left m Gamma) (at level 30).
-Notation "m :R Gamma" := (cons_Right m Gamma) (at level 30).
-Notation ":N Gamma" := (cons_Null Gamma) (at level 30).
+Notation "m :u Gamma" := (cons_u m Gamma) (at level 30).
+Notation "m :l Gamma" := (cons_l m Gamma) (at level 30).
+Notation "m :[ s ] Gamma" := (cons_s m s Gamma) (at level 30).
+Notation ":n Gamma" := (cons_n Gamma) (at level 30).
 
 Inductive merge T : context T -> context T -> context T -> Prop :=
 | merge_nil :
   merge nil nil nil
 | merge_left Gamma1 Gamma2 Gamma m : 
   merge Gamma1 Gamma2 Gamma ->
-  merge (m :L Gamma1) (m :L Gamma2) (m :L Gamma)
+  merge (m :u Gamma1) (m :u Gamma2) (m :u Gamma)
 | merge_right1 Gamma1 Gamma2 Gamma m :
   merge Gamma1 Gamma2 Gamma ->
-  merge (m :R Gamma1) (:N Gamma2) (m :R Gamma)
+  merge (m :l Gamma1) (:n Gamma2) (m :l Gamma)
 | merge_right2 Gamma1 Gamma2 Gamma m :
   merge Gamma1 Gamma2 Gamma ->
-  merge (:N Gamma1) (m :R Gamma2) (m :R Gamma)
+  merge (:n Gamma1) (m :l Gamma2) (m :l Gamma)
 | merge_null Gamma1 Gamma2 Gamma :
   merge Gamma1 Gamma2 Gamma ->
-  merge (:N Gamma1) (:N Gamma2) (:N Gamma).
+  merge (:n Gamma1) (:n Gamma2) (:n Gamma).
 
 Inductive pure T : context T -> Prop :=
 | pure_nil :
   pure nil
-| pure_L Gamma m : 
+| pure_u Gamma m : 
   pure Gamma ->
-  pure (m :L Gamma)
-| pure_N Gamma : 
+  pure (m :u Gamma)
+| pure_n Gamma : 
   pure Gamma ->
-  pure (:N Gamma).
+  pure (:n Gamma).
 
-Inductive ithR {T} : context T -> nat -> Prop :=
-| ithR_O m Gamma :
-  ithR (m :R Gamma) 0
-| ithR_S Gamma n e :
-  ithR Gamma n ->
-  ithR (e :: Gamma) n.+1.
+Inductive hasU {T} `{Ids T} `{Subst T} : 
+  context T -> var -> T -> Prop :=
+| hasU_O m Gamma :
+  pure Gamma ->
+  hasU (m :u Gamma) 0 m.[ren (+1)]
+| hasU_S Gamma v m n : 
+  hasU Gamma v m ->
+  hasU (n :u Gamma) (v.+1) m.[ren (+1)]
+| hasU_N Gamma v m : 
+  hasU Gamma v m ->
+  hasU (:n Gamma) (v.+1) m.[ren (+1)].
 
-Inductive ithL {T} : context T -> nat -> Prop :=
-| ithL_O m Gamma :
-  ithL (m :L Gamma) 0
-| ithL_S Gamma n e :
-  ithL Gamma n ->
-  ithL (e :: Gamma) n.+1.
-
-Inductive hasL {T} `{Ids T} `{Subst T} : 
+Inductive hasL {T} `{Ids T} `{Subst T} :
   context T -> var -> T -> Prop :=
 | hasL_O m Gamma :
   pure Gamma ->
-  hasL (m :L Gamma) 0 m.[ren (+1)]
-| hasL_S Gamma v m n : 
+  hasL (m :l Gamma) 0 m.[ren (+1)]
+| hasL_S Gamma v m n :
   hasL Gamma v m ->
-  hasL (n :L Gamma) (v.+1) m.[ren (+1)]
-| hasL_N Gamma v m : 
+  hasL (n :u Gamma) (v.+1) m.[ren (+1)]
+| hasL_N Gamma v m :
   hasL Gamma v m ->
-  hasL (:N Gamma) (v.+1) m.[ren (+1)].
-
-Inductive hasR {T} `{Ids T} `{Subst T} :
-  context T -> var -> T -> Prop :=
-| hasR_O m Gamma :
-  pure Gamma ->
-  hasR (m :R Gamma) 0 m.[ren (+1)]
-| hasR_S Gamma v m n :
-  hasR Gamma v m ->
-  hasR (n :L Gamma) (v.+1) m.[ren (+1)]
-| hasR_N Gamma v m :
-  hasR Gamma v m ->
-  hasR (:N Gamma) (v.+1) m.[ren (+1)].
+  hasL (:n Gamma) (v.+1) m.[ren (+1)].
 
 Fixpoint re T (Gamma : context T) : context T :=
   match Gamma with
-  | Left m :: Gamma => Left m :: re Gamma
-  | _ :: Gamma => Null _ :: re Gamma
+  | Some (m, U) :: Gamma => Some (m, U) :: re Gamma
+  | _ :: Gamma => None :: re Gamma
   | _ => nil
   end.
-
-Lemma ithR_pure T (Gamma : context T) n :
-  ithR Gamma n -> ~ pure Gamma.
-Proof.
-  unfold not.
-  intros.
-  induction H.
-  inv H0.
-  inv H0; eauto.
-Qed.
-
-Lemma hasR_ithR {T} `{Ids T} `{Subst T} (Gamma : context T) A n :
-  hasR Gamma n A -> forall m, ithR Gamma m -> m = n.
-Proof.
-  induction 1; intros.
-  - inv H2; eauto.
-    exfalso; eapply ithR_pure; eauto.
-  - inv H2.
-    erewrite <- IHhasR; eauto.
-  - inv H2.
-    erewrite <- IHhasR; eauto.
-Qed.
 
 Lemma merge_sym T (Gamma1 Gamma2 Gamma : context T) : 
   merge Gamma1 Gamma2 Gamma ->
@@ -220,12 +186,11 @@ Proof.
   - simpl.
     reflexivity.
   - case a; intros; simpl.
-    rewrite <- IHGamma.
-    reflexivity.
-    rewrite <- IHGamma.
-    reflexivity.
-    rewrite <- IHGamma.
-    reflexivity.
+    case p; intros; simpl.
+    case s; intros; simpl.
+    rewrite <- IHGamma; eauto.
+    rewrite <- IHGamma; eauto.
+    rewrite <- IHGamma; eauto.
 Qed.
 
 Lemma pure_re T (Gamma : context T) :
@@ -242,11 +207,16 @@ Lemma re_pure T (Gamma : context T) : pure (re Gamma).
 Proof.
   induction Gamma; intros.
   constructor.
-  destruct a; simpl; constructor; eauto.
+  destruct a; simpl. 
+  destruct p; simpl. 
+  destruct s; simpl. 
+  constructor; eauto.
+  constructor; eauto.
+  constructor; eauto.
 Qed.
 
-Lemma hasL_re {T} `{Ids T} `{Subst T} (Gamma : context T) x A :
-  hasL Gamma x A -> hasL (re Gamma) x A.
+Lemma hasU_re {T} `{Ids T} `{Subst T} (Gamma : context T) x A :
+  hasU Gamma x A -> hasU (re Gamma) x A.
 Proof.
   induction 1; simpl.
   - constructor.
@@ -255,18 +225,41 @@ Proof.
   - constructor; eauto.
 Qed.
 
-Lemma hasR_re {T} `{Ids T} `{Subst T} (Gamma : context T) :
-  forall x A, ~hasR (re Gamma) x A.
+Lemma hasL_re {T} `{Ids T} `{Subst T} (Gamma : context T) :
+  forall x A, ~hasL (re Gamma) x A.
 Proof.
   induction Gamma; unfold not; intros.
   - simpl in H1. inv H1.
-  - destruct a; simpl in H1; inv H1; eapply IHGamma; eauto.
+  - destruct a; inv H1. 
+    destruct p; inv H2. 
+    destruct s; inv H4. 
+    destruct p; inv H2. 
+    destruct s; inv H4. 
+    eapply IHGamma; eauto.
+    destruct p; inv H2. 
+    destruct s; inv H4. 
+    eapply IHGamma; eauto.
+    eapply IHGamma; eauto.
 Qed.
 
-Lemma hasL_pure {T} `{Ids T} `{Subst T} (Gamma : context T) x A :
-  hasL Gamma x A -> pure Gamma.
+Lemma hasU_pure {T} `{Ids T} `{Subst T} (Gamma : context T) x A :
+  hasU Gamma x A -> pure Gamma.
 Proof.
   induction 1; simpl; constructor; eauto.
+Qed.
+
+Lemma hasU_x {T} `{Ids T} `{Subst T} (Gamma : context T) x A :
+  hasU Gamma x A ->
+  forall B,
+    hasU Gamma x B ->
+    A = B.
+Proof.
+  induction 1; intros.
+  inv H2; eauto.
+  inv H2; eauto.
+  apply IHhasU in H7. rewrite H7; eauto.
+  inv H2; eauto.
+  apply IHhasU in H5. rewrite H5; eauto.
 Qed.
 
 Lemma hasL_x {T} `{Ids T} `{Subst T} (Gamma : context T) x A :
@@ -283,29 +276,15 @@ Proof.
   apply IHhasL in H5. rewrite H5; eauto.
 Qed.
 
-Lemma hasR_x {T} `{Ids T} `{Subst T} (Gamma : context T) x A :
-  hasR Gamma x A ->
+Lemma hasU_hasL {T} `{Ids T} `{Subst T} (Gamma : context T) x A :
+  hasU Gamma x A ->
   forall B,
-    hasR Gamma x B ->
-    A = B.
-Proof.
-  induction 1; intros.
-  inv H2; eauto.
-  inv H2; eauto.
-  apply IHhasR in H7. rewrite H7; eauto.
-  inv H2; eauto.
-  apply IHhasR in H5. rewrite H5; eauto.
-Qed.
-
-Lemma hasL_hasR {T} `{Ids T} `{Subst T} (Gamma : context T) x A :
-  hasL Gamma x A ->
-  forall B,
-    ~ hasR Gamma x B.
+    ~ hasL Gamma x B.
 Proof.
   induction 1; unfold not; intros.
   inv H2.
-  inv H2; apply IHhasL in H7; eauto.
-  inv H2; apply IHhasL in H5; eauto.
+  inv H2; apply IHhasU in H7; eauto.
+  inv H2; apply IHhasU in H5; eauto.
 Qed.
 
 Lemma merge_split1 T (Gamma1 Gamma2 Gamma : context T) :
@@ -323,26 +302,26 @@ Proof.
   - inv H0.
     specialize (IHmerge _ _ H4).
     firstorder.
-    exists (m :L x).
+    exists (m :u x).
     repeat constructor; eauto.
   - inv H0.
     + specialize (IHmerge _ _ H4).
       firstorder.
-      exists (m :R x).
+      exists (m :l x).
       repeat constructor; eauto.
     + specialize (IHmerge _ _ H4).
       firstorder.
-      exists (:N x).
+      exists (:n x).
       repeat constructor; eauto.
   - inv H0.
     specialize (IHmerge _ _ H4).
     firstorder.
-    exists (m :R x).
+    exists (m :l x).
     repeat constructor; eauto.
   - inv H0.
     specialize (IHmerge _ _ H4).
     firstorder.
-    exists (:N x).
+    exists (:n x).
     repeat constructor; eauto.
 Qed.
 
@@ -361,34 +340,32 @@ Proof.
   - inv H0.
     specialize (IHmerge _ _ H4).
     firstorder.
-    exists (m :L x).
+    exists (m :u x).
     repeat constructor; eauto.
   - inv H0.
     + specialize (IHmerge _ _ H4).
       firstorder.
-      exists (:N x).
+      exists (:n x).
       repeat constructor; eauto.
     + specialize (IHmerge _ _ H4).
       firstorder.
-      exists (m :R x).
+      exists (m :l x).
       repeat constructor; eauto.
   - inv H0.
     specialize (IHmerge _ _ H4).
     firstorder.
-    exists (m :R x).
+    exists (m :l x).
     repeat constructor; eauto.
   - inv H0.
     specialize (IHmerge _ _ H4).
     firstorder.
-    exists (:N x).
+    exists (:n x).
     repeat constructor; eauto.
 Qed.
 
-Inductive sort : Type := U | L.
-
 Inductive term : Type :=
 | Var    (x : var)
-| Sort   (srt : sort) (l : nat)
+| Sort   (s : sort)
 | TyProd (A : term) (B : {bind term}) (s : sort)
 | LnProd (A : term) (B : {bind term}) (s : sort)
 | Arrow  (A B : term) (s : sort)
@@ -402,7 +379,7 @@ Instance Subst_term : Subst term. derive. Defined.
 Instance substLemmas_term : SubstLemmas term. derive. Qed.
 
 Inductive value : term -> Prop :=
-| value_sort srt l   : value (Sort srt l)
+| value_sort s       : value (Sort s)
 | value_var x        : value (Var x)
 | value_tyProd A B s : value (TyProd A B s)
 | value_lnProd A B s : value (LnProd A B s)
@@ -478,8 +455,8 @@ Inductive step : term -> term -> Prop :=
 Inductive pstep : term -> term -> Prop :=
 | pstep_var x :
   pstep (Var x) (Var x)
-| pstep_sort srt l :
-  pstep (Sort srt l) (Sort srt l)
+| pstep_sort s :
+  pstep (Sort s) (Sort s)
 | pstep_lam n n' : 
   pstep n n' -> 
   pstep (Lam n) (Lam n')
@@ -672,7 +649,7 @@ Proof with eauto using pstep.
   intros.
   dependent induction H.
   - inv H0. exists (Var x)...
-  - inv H0. exists (Sort srt l)...
+  - inv H0. exists (Sort s)...
   - inv H0. apply (IHpstep) in H2. first_order. exists (Lam x)...
   - inv H1.
     + apply (IHpstep1) in H4. apply (IHpstep2) in H6. first_order.
@@ -771,8 +748,8 @@ Proof.
   apply rename_v_subst.
 Qed.
 
-Lemma sort_ren_inv s l v xi :
-  Sort s l = v.[ren xi] -> v = Sort s l.
+Lemma sort_ren_inv s v xi :
+  Sort s = v.[ren xi] -> v = Sort s.
 Proof.
   induction v; asimpl; try discriminate; eauto.
 Qed.
@@ -832,212 +809,102 @@ Proof.
   apply lam_ren_inv in x; inv x; constructor.
 Qed.
 
-Definition left_invertible (f : nat -> nat) := 
-  exists g, g ∘ f = id.
+Reserved Notation "[ Gamma |- ]".
+Reserved Notation "[ Gamma |- m :- A -: s ]".
 
-Lemma left_invertible_upren xi :
-  left_invertible xi -> left_invertible (upren xi).
-Proof.
-  unfold left_invertible.
-  intros.
-  inv H.
-  exists (upren x).
-  assert (upren x ∘ upren xi = upren xi >>> upren x) by autosubst.
-  rewrite H; asimpl.
-  replace (xi >>> x) with (x ∘ xi) by autosubst.
-  rewrite H0; autosubst.
-Qed.
-
-Lemma pstep_ren_inv m n xi :
-  pstep m.[ren xi] n ->
-  left_invertible xi ->
-    exists x, pstep m x /\ x.[ren xi] = n.
-Proof.
-  intro H.
-  dependent induction H; intros.
-  - inv H.
-    exists ((Var x0).[ren x1]).
-    rewrite x; asimpl.
-    replace (xi >>> x1) with (x1 ∘ xi) by autosubst.
-    rewrite H0; asimpl; firstorder.
-    apply pstep_refl.
-  - exists m; firstorder.
-    apply pstep_refl.
-  - destruct m; asimpl; try discriminate.
-    inversion H0.
-    inv x.
-    assert (n0.[up (ren xi)] = n0.[ren (upren xi)]) by autosubst.
-    apply left_invertible_upren in H0.
-    pose proof (IHpstep n0 (upren xi) H2 H0).
-    inv H3. inv H4.
-    exists (Lam x); asimpl; firstorder.
-    constructor; eauto.
-  - destruct m; asimpl; try discriminate. inv x.
-    assert (m1.[ren xi] = m1.[ren xi]) by eauto.
-    assert (m2.[ren xi] = m2.[ren xi]) by eauto.
-    apply IHpstep1 in H2; eauto.
-    apply IHpstep2 in H3; eauto.
-    firstorder; subst; asimpl.
-    exists (App x1 x).
-    firstorder.
-    constructor; eauto.
-  - destruct m; asimpl; try discriminate. inv x.
-    destruct m1; asimpl; try discriminate. inv H4.
-    assert (n0.[up (ren xi)] = n0.[ren (upren xi)]) by autosubst.
-    pose proof (left_invertible_upren H2).
-    pose proof (IHpstep1 n0 (upren xi) H3 H4).
-    assert (m2.[ren xi] = m2.[ren xi]) by eauto.
-    pose proof (IHpstep2 m2 xi H6 H2).
-    firstorder; subst; asimpl.
-    exists (x1.[x .: ids]); asimpl.
-    firstorder.
-    constructor; eauto.
-    apply <- value_rename; eauto.
-  - destruct m; asimpl; try discriminate. inv x.
-    assert (m.[ren xi] = m.[ren xi]) by eauto.
-    assert (B0.[up (ren xi)] = B0.[ren (upren xi)]) by autosubst.
-    assert (left_invertible (upren xi)).
-    apply left_invertible_upren; eauto.
-    apply IHpstep1 in H2; eauto.
-    apply IHpstep2 in H3; eauto.
-    firstorder; subst; asimpl.
-    exists (TyProd x0 x1 s0); asimpl; firstorder.
-    constructor; eauto.
-  - destruct m; asimpl; try discriminate. inv x.
-    assert (m.[ren xi] = m.[ren xi]) by eauto.
-    assert (B0.[up (ren xi)] = B0.[ren (upren xi)]) by autosubst.
-    assert (left_invertible (upren xi)).
-    apply left_invertible_upren; eauto.
-    apply IHpstep1 in H2; eauto.
-    apply IHpstep2 in H3; eauto.
-    firstorder; subst; asimpl.
-    exists (LnProd x0 x1 s0); asimpl; firstorder.
-    constructor; eauto.
-  - destruct m; asimpl; try discriminate. inv x.
-    assert (m1.[ren xi] = m1.[ren xi]) by eauto.
-    assert (m2.[ren xi] = m2.[ren xi]) by eauto.
-    apply IHpstep1 in H2; eauto.
-    apply IHpstep2 in H3; eauto.
-    firstorder; subst; asimpl.
-    exists (Arrow x1 x s0); asimpl; firstorder.
-    constructor; eauto.
-  - destruct m; asimpl; try discriminate. inv x.
-    assert (m1.[ren xi] = m1.[ren xi]) by eauto.
-    assert (m2.[ren xi] = m2.[ren xi]) by eauto.
-    apply IHpstep1 in H2; eauto.
-    apply IHpstep2 in H3; eauto.
-    firstorder; subst; asimpl.
-    exists (Lolli x1 x s0); asimpl; firstorder.
-    constructor; eauto.
-Qed.
-
-Lemma pstep_ren1_inv m n :
-  pstep m.[ren (+1)] n ->
-    exists x, pstep m x /\ x.[ren (+1)] = n.
-Proof.
-  intros.
-  apply pstep_ren_inv; eauto.
-  unfold left_invertible.
-  exists (predn).
-  autosubst.
-Qed.
-
-Reserved Notation "[ Gamma |= ]".
-Reserved Notation "[ Gamma |= m :- A -: s ]".
-  
 Inductive has_type : context term -> term -> term -> sort -> Prop :=
-| axiom Gamma s l : 
+| axiom Gamma s : 
   pure Gamma ->
-  [ Gamma |= Sort s l :- Sort U l.+1 -: U ]
-| u_prod Gamma A B s l :
+  [ Gamma |- Sort s :- Sort U -: U ]
+| u_prod Gamma A B s :
   pure Gamma ->
-  [ Gamma |= A :- Sort U l -: U ] ->
-  [ A :L Gamma |= B :- Sort s l -: U ] ->
-  [ Gamma |= TyProd A B s :- Sort U l -: U ]
-| l_prod Gamma A B s l :
+  [ Gamma |- A :- Sort U -: U ] ->
+  [ A :u Gamma |- B :- Sort s -: U ] ->
+  [ Gamma |- TyProd A B s :- Sort U -: U ]
+| l_prod Gamma A B s :
   pure Gamma ->
-  [ Gamma |= A :- Sort U l -: U ] ->
-  [ A :L Gamma |= B :- Sort s l -: U ] ->
-  [ Gamma |= LnProd A B s :- Sort L l -: U ]
-| arrow Gamma A B s l :
+  [ Gamma |- A :- Sort U -: U ] ->
+  [ A :u Gamma |- B :- Sort s -: U ] ->
+  [ Gamma |- LnProd A B s :- Sort L -: U ]
+| arrow Gamma A B s :
   pure Gamma ->
-  [ Gamma |= A :- Sort L l -: U ] ->
-  [ Gamma |= B :- Sort s l -: U ] ->
-  [ Gamma |= Arrow A B s :- Sort U l -: U ]
-| lolli Gamma A B s l :
+  [ Gamma |- A :- Sort L -: U ] ->
+  [ Gamma |- B :- Sort s -: U ] ->
+  [ Gamma |- Arrow A B s :- Sort U -: U ]
+| lolli Gamma A B s :
   pure Gamma ->
-  [ Gamma |= A :- Sort L l -: U ] ->
-  [ Gamma |= B :- Sort s l -: U ] ->
-  [ Gamma |= Lolli A B s :- Sort L l -: U ]
+  [ Gamma |- A :- Sort L -: U ] ->
+  [ Gamma |- B :- Sort s -: U ] ->
+  [ Gamma |- Lolli A B s :- Sort L -: U ]
 | u_var Gamma x A : 
-  hasL Gamma x A ->
-  [ Gamma |= Var x :- A -: U ]
+  hasU Gamma x A ->
+  [ Gamma |- Var x :- A -: U ]
 | l_var Gamma x A :
-  hasR Gamma x A ->
-  [ Gamma |= Var x :- A -: L ]
-| u_lam1 Gamma n A B s l :
+  hasL Gamma x A ->
+  [ Gamma |- Var x :- A -: L ]
+| u_lam1 Gamma n A B s :
   pure Gamma ->
-  [ Gamma |= TyProd A B s :- Sort U l -: U ] ->
-  [ A :L Gamma |= n :- B -: s ] ->
-  [ Gamma |= Lam n :- TyProd A B s -: U ]
-| u_lam2 Gamma n A B s l :
+  [ Gamma |- TyProd A B s :- Sort U -: U ] ->
+  [ A :u Gamma |- n :- B -: s ] ->
+  [ Gamma |- Lam n :- TyProd A B s -: U ]
+| u_lam2 Gamma n A B s :
   pure Gamma ->
-  [ Gamma |= Arrow A B s :- Sort U l -: U ] ->
-  [ A :R Gamma |= n :- B.[ren (+1)] -: s ] ->
-  [ Gamma |= Lam n :- Arrow A B s -: U ]
-| l_lam1 Gamma n A B s l :
-  [ re Gamma |= LnProd A B s :- Sort L l -: U ] ->
-  [ A :L Gamma |= n :- B -: s ] ->
-  [ Gamma |= Lam n :- LnProd A B s -: L ]
-| l_lam2 Gamma n A B s l :
-  [ re Gamma |= Lolli A B s :- Sort L l -: U ] ->
-  [ A :R Gamma |= n :- B.[ren (+1)] -: s ] ->
-  [ Gamma |= Lam n :- Lolli A B s -: L ]
+  [ Gamma |- Arrow A B s :- Sort U -: U ] ->
+  [ A :l Gamma |- n :- B.[ren (+1)] -: s ] ->
+  [ Gamma |- Lam n :- Arrow A B s -: U ]
+| l_lam1 Gamma n A B s :
+  [ re Gamma |- LnProd A B s :- Sort L -: U ] ->
+  [ A :u Gamma |- n :- B -: s ] ->
+  [ Gamma |- Lam n :- LnProd A B s -: L ]
+| l_lam2 Gamma n A B s :
+  [ re Gamma |- Lolli A B s :- Sort L -: U ] ->
+  [ A :l Gamma |- n :- B.[ren (+1)] -: s ] ->
+  [ Gamma |- Lam n :- Lolli A B s -: L ]
 | u_app1 Gamma1 Gamma2 Gamma A B m n s :
-  [ Gamma1 |= m :- TyProd A B s -: U ] ->
-  [ Gamma2 |= n :- A -: U ] ->
+  [ Gamma1 |- m :- TyProd A B s -: U ] ->
+  [ Gamma2 |- n :- A -: U ] ->
   merge Gamma1 Gamma2 Gamma ->
-  [ Gamma |= App m n :- App (Lam B) n -: s ]
+  [ Gamma |- App m n :- App (Lam B) n -: s ]
 | u_app2 Gamma1 Gamma2 Gamma A B m n s :
-  [ Gamma1 |= m :- Arrow A B s -: U ] ->
-  [ Gamma2 |= n :- A -: L ] ->
+  [ Gamma1 |- m :- Arrow A B s -: U ] ->
+  [ Gamma2 |- n :- A -: L ] ->
   merge Gamma1 Gamma2 Gamma ->
-  [ Gamma |= App m n :- B -: s ]
+  [ Gamma |- App m n :- B -: s ]
 | l_app1 Gamma1 Gamma2 Gamma A B m n s :
-  [ Gamma1 |= m :- LnProd A B s -: L ] ->
-  [ Gamma2 |= n :- A -: U ] ->
+  [ Gamma1 |- m :- LnProd A B s -: L ] ->
+  [ Gamma2 |- n :- A -: U ] ->
   merge Gamma1 Gamma2 Gamma ->
-  [ Gamma |= App m n :- App (Lam B) n -: s ]
+  [ Gamma |- App m n :- App (Lam B) n -: s ]
 | l_app2 Gamma1 Gamma2 Gamma A B m n s :
-  [ Gamma1 |= m :- Lolli A B s -: L ] ->
-  [ Gamma2 |= n :- A -: L ] ->
+  [ Gamma1 |- m :- Lolli A B s -: L ] ->
+  [ Gamma2 |- n :- A -: L ] ->
   merge Gamma1 Gamma2 Gamma ->
-  [ Gamma |= App m n :- B -: s ]
+  [ Gamma |- App m n :- B -: s ]
 | conversion Gamma A B m s :
   A === B ->
-  [ Gamma |= m :- A -: s ] ->
-  [ Gamma |= m :- B -: s ]
-where "[ Gamma |= m :- A -: s ]" := (has_type Gamma m A s).
+  [ Gamma |- m :- A -: s ] ->
+  [ Gamma |- m :- B -: s ]
+where "[ Gamma |- m :- A -: s ]" := (has_type Gamma m A s).
 
 Inductive context_ok : context term -> Prop :=
 | nil_ok :
-  [ nil |= ]
-| u_ok Gamma A l :
-  [ Gamma |= ] ->
-  [ re Gamma |= A :- Sort U l -: U ] ->
-  [ A :L Gamma |= ]
-| l_ok Gamma A l :
-  [ Gamma |= ] ->
-  [ re Gamma |= A :- Sort L l -: U ] ->
-  [ A :R Gamma |= ]
+  [ nil |- ]
+| u_ok Gamma A :
+  [ Gamma |- ] ->
+  [ re Gamma |- A :- Sort U -: U ] ->
+  [ A :u Gamma |- ]
+| l_ok Gamma A :
+  [ Gamma |- ] ->
+  [ re Gamma |- A :- Sort L -: U ] ->
+  [ A :l Gamma |- ]
 | n_ok Gamma :
-  [ Gamma |= ] ->
-  [ :N Gamma |= ]
-where "[ Gamma |= ]" := (context_ok Gamma).
+  [ Gamma |- ] ->
+  [ :n Gamma |- ]
+where "[ Gamma |- ]" := (context_ok Gamma).
 
 Lemma re_ok Gamma :
-  [ Gamma |= ] ->
-  [ re Gamma |= ].
+  [ Gamma |- ] ->
+  [ re Gamma |- ].
 Proof with eauto using context_ok.
   intros.
   induction H...
@@ -1056,21 +923,21 @@ Inductive agree_ren : (var -> var) ->
   context term -> context term -> Prop :=
 | agree_ren_nil xi :
   agree_ren xi nil nil
-| agree_ren_L Gamma Gamma' xi m :
+| agree_ren_u Gamma Gamma' xi m :
   agree_ren xi Gamma Gamma' ->
-  agree_ren (upren xi) (m :L Gamma) (m.[ren xi] :L Gamma')
-| agree_ren_R Gamma Gamma' xi m :
+  agree_ren (upren xi) (m :u Gamma) (m.[ren xi] :u Gamma')
+| agree_ren_l Gamma Gamma' xi m :
   agree_ren xi Gamma Gamma' ->
-  agree_ren (upren xi) (m :R Gamma) (m.[ren xi] :R Gamma')
-| agree_ren_N Gamma Gamma' xi :
+  agree_ren (upren xi) (m :l Gamma) (m.[ren xi] :l Gamma')
+| agree_ren_n Gamma Gamma' xi :
   agree_ren xi Gamma Gamma' ->
-  agree_ren (upren xi) (:N Gamma) (:N Gamma')
-| agree_ren_wkL Gamma Gamma' xi m :
+  agree_ren (upren xi) (:n Gamma) (:n Gamma')
+| agree_ren_wkU Gamma Gamma' xi m :
   agree_ren xi Gamma Gamma' ->
-  agree_ren ((+1) ∘ xi) (Gamma) (m :L Gamma')
+  agree_ren ((+1) ∘ xi) (Gamma) (m :u Gamma')
 | agree_ren_wkN Gamma Gamma' xi :
   agree_ren xi Gamma Gamma' ->
-  agree_ren ((+1) ∘ xi) (Gamma) (:N Gamma').
+  agree_ren ((+1) ∘ xi) (Gamma) (:n Gamma').
 
 Lemma agree_ren_refl Gamma :
   agree_ren id Gamma Gamma.
@@ -1078,17 +945,22 @@ Proof.
   induction Gamma.
   - constructor.
   - destruct a. 
-    replace (agree_ren id (Left t :: Gamma) (Left t :: Gamma))
-      with (agree_ren (upren id) (t :L Gamma) (t.[ren id] :L Gamma))
+    destruct p.
+    destruct s.
+    assert (agree_ren id (t :u Gamma) (t :u Gamma)
+      = agree_ren (upren id) (t :u Gamma) (t.[ren id] :u Gamma))
       by autosubst.
+    rewrite H.
     constructor; eauto.
-    replace (agree_ren id (Right t :: Gamma) (Right t :: Gamma))
-      with (agree_ren (upren id) (t :R Gamma) (t.[ren id] :R Gamma))
+    assert (agree_ren id (t :l Gamma) (t :l Gamma)
+      = agree_ren (upren id) (t :l Gamma) (t.[ren id] :l Gamma))
       by autosubst.
+    rewrite H.
     constructor; eauto.
-    replace (agree_ren id (Null _ :: Gamma) (Null _ :: Gamma))
-      with (agree_ren (upren id) (:N Gamma) (:N Gamma))
+    assert (agree_ren id (:n Gamma) (:n Gamma)
+      = agree_ren (upren id) (:n Gamma) (:n Gamma))
       by autosubst.
+    rewrite H.
     constructor; eauto.
 Qed.
 
@@ -1114,11 +986,11 @@ Proof.
   induction 1; simpl; constructor; eauto.
 Qed.
 
-Lemma agree_ren_hasL Gamma Gamma' xi :
+Lemma agree_ren_hasU Gamma Gamma' xi :
   agree_ren xi Gamma Gamma' ->
   forall x A,
-    hasL Gamma x A ->
-    hasL Gamma' (xi x) A.[ren xi].
+    hasU Gamma x A ->
+    hasU Gamma' (xi x) A.[ren xi].
 Proof.
   intro H2.
   dependent induction H2; simpl; intros; eauto.
@@ -1150,11 +1022,11 @@ Proof.
     apply IHagree_ren; eauto.
 Qed.
 
-Lemma agree_ren_hasR Gamma Gamma' xi :
+Lemma agree_ren_hasL Gamma Gamma' xi :
   agree_ren xi Gamma Gamma' ->
   forall x A,
-    hasR Gamma x A ->
-    hasR Gamma' (xi x) A.[ren xi].
+    hasL Gamma x A ->
+    hasL Gamma' (xi x) A.[ren xi].
 Proof.
   intro H2.
   dependent induction H2; simpl; intros; eauto.
@@ -1203,43 +1075,43 @@ Proof.
   - inv H0; subst.
     pose proof (IHagree_ren _ _ H4).
     first_order.
-    exists (m.[ren xi] :L x).
-    exists (m.[ren xi] :L x0).
+    exists (m.[ren xi] :u x).
+    exists (m.[ren xi] :u x0).
     repeat constructor; eauto.
   - inv H0; subst.
     pose proof (IHagree_ren _ _ H4).
     first_order.
-    exists (m.[ren xi] :R x).
-    exists (:N x0).
+    exists (m.[ren xi] :l x).
+    exists (:n x0).
     repeat constructor; eauto.
     pose proof (IHagree_ren _ _ H4).
     first_order.
-    exists (:N x).
-    exists (m.[ren xi] :R x0).
+    exists (:n x).
+    exists (m.[ren xi] :l x0).
     repeat constructor; eauto.
   - inv H0; subst.
     pose proof (IHagree_ren _ _ H4).
     first_order.
-    exists (:N x).
-    exists (:N x0).
+    exists (:n x).
+    exists (:n x0).
     repeat constructor; eauto.
   - pose proof (IHagree_ren _ _ H0).
     first_order.
-    exists (m :L x).
-    exists (m :L x0).
+    exists (m :u x).
+    exists (m :u x0).
     repeat constructor; eauto.
   - pose proof (IHagree_ren _ _ H0).
     first_order.
-    exists (:N x).
-    exists (:N x0).
+    exists (:n x).
+    exists (:n x0).
     repeat constructor; eauto.
 Qed.
 
 Lemma rename_ok Gamma m A s :
-  [ Gamma |= m :- A -: s ] ->
+  [ Gamma |- m :- A -: s ] ->
   forall Gamma' xi,
     agree_ren xi Gamma Gamma' ->
-    [ Gamma' |= m.[ren xi] :- A.[ren xi] -: s ].
+    [ Gamma' |- m.[ren xi] :- A.[ren xi] -: s ].
 Proof.
   intros H.
   induction H; simpl; intros.
@@ -1248,13 +1120,13 @@ Proof.
   - asimpl.
     pose proof (agree_ren_pure H2 H).
     apply u_prod; eauto.
-    replace (Sort s l) with ((Sort s l).[ren (upren xi)]) by autosubst.
+    replace (Sort s) with ((Sort s).[ren (upren xi)]) by autosubst.
     apply IHhas_type2.
     constructor; eauto.
   - asimpl.
     pose proof (agree_ren_pure H2 H).
     apply l_prod; eauto.
-    replace (Sort s l) with ((Sort s l).[ren (upren xi)]) by autosubst.
+    replace (Sort s) with ((Sort s).[ren (upren xi)]) by autosubst.
     apply IHhas_type2.
     constructor; eauto.
   - asimpl.
@@ -1265,10 +1137,10 @@ Proof.
     apply lolli; eauto.
   - replace (ids (xi x)) with (Var (xi x)) by autosubst.
     apply u_var.
-    eapply agree_ren_hasL; eauto.
+    eapply agree_ren_hasU; eauto.
   - replace (ids (xi x)) with (Var (xi x)) by autosubst.
     apply l_var.
-    eapply agree_ren_hasR; eauto.
+    eapply agree_ren_hasL; eauto.
   - eapply u_lam1.
     eapply agree_ren_pure; eauto.
     apply IHhas_type1; eauto.
@@ -1316,74 +1188,59 @@ Proof.
     apply IHhas_type; eauto.
 Qed.
 
-Lemma hasL_ok Gamma :
-  [ Gamma |= ] ->
+Lemma hasU_ok Gamma :
+  [ Gamma |- ] ->
   forall x A,
-    hasL Gamma x A ->
-    exists l, [ re Gamma |= A :- Sort U l -: U ].
+    hasU Gamma x A -> [ re Gamma |- A :- Sort U -: U ].
 Proof.
   induction 1; intros.
   - inv H.
   - inv H1; simpl.
-    exists l.
-    replace (Sort U l) with ((Sort U l).[ren (+1)]) by autosubst.
+    replace (Sort U) with ((Sort U).[ren (+1)]) by autosubst.
     eapply rename_ok.
     apply H0.
-    apply agree_ren_wkL.
+    apply agree_ren_wkU.
     rewrite <- pure_re; eauto.
     apply agree_ren_refl.
-    specialize (IHcontext_ok _ _ H6).
-    inv IHcontext_ok.
-    exists x.
-    replace (Sort U x) with ((Sort U x).[ren (+1)]) by autosubst.
+    replace (Sort U) with ((Sort U).[ren (+1)]) by autosubst.
     eapply rename_ok; eauto.
-    apply agree_ren_wkL.
+    apply agree_ren_wkU.
     apply agree_ren_refl.
   - inv H1.
   - inv H0.
     specialize (IHcontext_ok _ _ H2).
-    inv IHcontext_ok.
-    exists x.
-    replace (Sort U x) with ((Sort U x).[ren (+1)]) by autosubst.
+    replace (Sort U) with ((Sort U).[ren (+1)]) by autosubst.
     eapply rename_ok; eauto.
     apply agree_ren_wkN.
     apply agree_ren_refl.
 Qed.
 
 Lemma hasR_ok Gamma :
-  [ Gamma |= ] ->
+  [ Gamma |- ] ->
   forall x A,
-    hasR Gamma x A ->
-    exists l, [ re Gamma |= A :- Sort L l -: U ].
+    hasL Gamma x A -> [ re Gamma |- A :- Sort L -: U ].
 Proof.
   induction 1; intros.
   - inv H.
   - inv H1; simpl.
-    specialize (IHcontext_ok _ _ H6).
-    inv IHcontext_ok.
-    exists x.
-    replace (Sort L x) with ((Sort L x).[ren (+1)]) by autosubst.
+    replace (Sort L) with ((Sort L).[ren (+1)]) by autosubst.
     eapply rename_ok; eauto.
-    apply agree_ren_wkL.
+    apply agree_ren_wkU.
     apply agree_ren_refl.
   - inv H1; simpl.
-    exists l.
-    replace (Sort L l) with ((Sort L l).[ren (+1)]) by autosubst.
+    replace (Sort L) with ((Sort L).[ren (+1)]) by autosubst.
     eapply rename_ok; eauto.
     apply agree_ren_wkN.
     apply agree_ren_refl.
   - inv H0; simpl.
-    specialize (IHcontext_ok _ _ H2).
-    inv IHcontext_ok.
-    exists x.
-    replace (Sort L x) with ((Sort L x).[ren (+1)]) by autosubst.
+    replace (Sort L) with ((Sort L).[ren (+1)]) by autosubst.
     eapply rename_ok; eauto.
     apply agree_ren_wkN.
     apply agree_ren_refl.
 Qed.
 
-Lemma red_sort_inv s l A :
-  red (Sort s l) A -> A = (Sort s l).
+Lemma red_sort_inv s A :
+  red (Sort s) A -> A = (Sort s).
 Proof.
   induction 1; intros; eauto.
   rewrite IHstar in H0.
@@ -1488,31 +1345,31 @@ Proof.
 Qed.
 
 Lemma value_sound Gamma m A :
-  [ Gamma |= m :- A -: U ] -> value m -> pure Gamma.
+  [ Gamma |- m :- A -: U ] -> value m -> pure Gamma.
 Proof.
   intros H.
   dependent induction H; intros; eauto.
-  - eapply hasL_pure; eauto.
+  - eapply hasU_pure; eauto.
   - inv H2.
   - inv H2.
   - inv H2.
   - inv H2.
 Qed.
 
-Lemma weakening_L Gamma m A s B :
-  [ Gamma |= m :- A -: s ] ->
-  [ B :L Gamma |= m.[ren (+1)] :- A.[ren (+1)] -: s ].
+Lemma weakening_u Gamma m A s B :
+  [ Gamma |- m :- A -: s ] ->
+  [ B :u Gamma |- m.[ren (+1)] :- A.[ren (+1)] -: s ].
 Proof.
   intros.
   eapply rename_ok in H.
   apply H.
-  apply agree_ren_wkL.
+  apply agree_ren_wkU.
   apply agree_ren_refl.
 Qed.
 
-Lemma weakening_N Gamma m A s :
-  [ Gamma |= m :- A -: s ] ->
-  [ :N Gamma |= m.[ren (+1)] :- A.[ren (+1)] -: s ].
+Lemma weakening_n Gamma m A s :
+  [ Gamma |- m :- A -: s ] ->
+  [ :n Gamma |- m.[ren (+1)] :- A.[ren (+1)] -: s ].
 Proof.
   intros.
   eapply rename_ok in H.
@@ -1521,69 +1378,69 @@ Proof.
   apply agree_ren_refl.
 Qed.
 
-Lemma eweakening_L Gamma m m' A A' s B :
+Lemma eweakening_u Gamma m m' A A' s B :
   m' = m.[ren (+1)] -> 
   A' = A.[ren (+1)] ->
-  [ Gamma |= m :- A -: s ] -> 
-  [ B :L Gamma |= m' :- A' -: s ].
+  [ Gamma |- m :- A -: s ] -> 
+  [ B :u Gamma |- m' :- A' -: s ].
 Proof.  
   intros; subst.
-  apply weakening_L; eauto.
+  apply weakening_u; eauto.
 Qed.
 
-Lemma eweakening_N Gamma m m' A A' s :
+Lemma eweakening_n Gamma m m' A A' s :
   m' = m.[ren (+1)] -> 
   A' = A.[ren (+1)] ->
-  [ Gamma |= m :- A -: s ] -> 
-  [ :N Gamma |= m' :- A' -: s ].
+  [ Gamma |- m :- A -: s ] -> 
+  [ :n Gamma |- m' :- A' -: s ].
 Proof.  
   intros; subst.
-  apply weakening_N; eauto.
+  apply weakening_n; eauto.
 Qed.
 
-Reserved Notation "[ Delta |= sigma -| Gamma ]".
+Reserved Notation "[ Delta |- sigma -| Gamma ]".
 
 Inductive agree_subst :
   context term -> (var -> term) -> context term -> Prop :=
 | agree_subst_nil sigma :
   v_subst sigma ->
-  [ nil |= sigma -| nil ]
-| agree_subst_L Delta sigma Gamma A :
-  [ Delta |= sigma -| Gamma ] ->
-  [ A.[sigma] :L Delta |= up sigma -| A :L Gamma ]
-| agree_subst_R Delta sigma Gamma A :
-  [ Delta |= sigma -| Gamma ] ->
-  [ A.[sigma] :R Delta |= up sigma -| A :R Gamma ]
-| agree_subst_N Delta sigma Gamma :
-  [ Delta |= sigma -| Gamma ] ->
-  [ :N Delta |= up sigma -| :N Gamma ]
-| agree_subst_wkL Delta sigma Gamma n A :
+  [ nil |- sigma -| nil ]
+| agree_subst_u Delta sigma Gamma A :
+  [ Delta |- sigma -| Gamma ] ->
+  [ A.[sigma] :u Delta |- up sigma -| A :u Gamma ]
+| agree_subst_l Delta sigma Gamma A :
+  [ Delta |- sigma -| Gamma ] ->
+  [ A.[sigma] :l Delta |- up sigma -| A :l Gamma ]
+| agree_subst_n Delta sigma Gamma :
+  [ Delta |- sigma -| Gamma ] ->
+  [ :n Delta |- up sigma -| :n Gamma ]
+| agree_subst_wkU Delta sigma Gamma n A :
   value n ->
-  [ Delta |= sigma -| Gamma ] ->
-  [ re Delta |= n :- A.[sigma] -: U ] ->
-  [ Delta |= n .: sigma -| A :L Gamma ]
-| agree_subst_wkR Delta1 Delta2 Delta sigma Gamma n A :
+  [ Delta |- sigma -| Gamma ] ->
+  [ re Delta |- n :- A.[sigma] -: U ] ->
+  [ Delta |- n .: sigma -| A :u Gamma ]
+| agree_subst_wkL Delta1 Delta2 Delta sigma Gamma n A :
   value n ->
   merge Delta1 Delta2 Delta ->
-  [ Delta1 |= sigma -| Gamma ] ->
-  [ Delta2 |= n :- A.[sigma] -: L ] ->
-  [ Delta |= n .: sigma -| A :R Gamma ]
+  [ Delta1 |- sigma -| Gamma ] ->
+  [ Delta2 |- n :- A.[sigma] -: L ] ->
+  [ Delta |- n .: sigma -| A :l Gamma ]
 | agree_subst_wkN Delta sigma Gamma n :
   value n ->
-  [ Delta |= sigma -| Gamma ] ->
-  [ Delta |= n .: sigma -| :N Gamma ]
+  [ Delta |- sigma -| Gamma ] ->
+  [ Delta |- n .: sigma -| :n Gamma ]
+| agree_subst_convU Delta sigma Gamma A B :
+  A === B ->
+  [ Delta |- sigma -| A :u Gamma ] ->
+  [ Delta |- sigma -| B :u Gamma ]
 | agree_subst_convL Delta sigma Gamma A B :
   A === B ->
-  [ Delta |= sigma -| A :L Gamma ] ->
-  [ Delta |= sigma -| B :L Gamma ]
-| agree_subst_convR Delta sigma Gamma A B :
-  A === B ->
-  [ Delta |= sigma -| A :R Gamma ] ->
-  [ Delta |= sigma -| B :R Gamma ]
-where "[ Delta |= sigma -| Gamma ]" := (agree_subst Delta sigma Gamma).
+  [ Delta |- sigma -| A :l Gamma ] ->
+  [ Delta |- sigma -| B :l Gamma ]
+where "[ Delta |- sigma -| Gamma ]" := (agree_subst Delta sigma Gamma).
 
 Lemma agree_subst_v_subst Delta sigma Gamma :
-  [ Delta |= sigma -| Gamma ] -> v_subst sigma.
+  [ Delta |- sigma -| Gamma ] -> v_subst sigma.
 Proof.
   induction 1; intros; eauto.
   - apply v_subst_up; eauto.
@@ -1595,7 +1452,7 @@ Proof.
 Qed.
 
 Lemma agree_subst_pure Delta sigma Gamma :
-  [ Delta |= sigma -| Gamma ] -> pure Gamma -> pure Delta.
+  [ Delta |- sigma -| Gamma ] -> pure Gamma -> pure Delta.
 Proof.
   induction 1; intros; eauto.
   inv H0.
@@ -1613,29 +1470,31 @@ Proof.
 Qed.
 
 Lemma agree_subst_refl Gamma :
-  [ Gamma |= ids -| Gamma ].
+  [ Gamma |- ids -| Gamma ].
 Proof.
   induction Gamma.
   - constructor.
     apply ids_v_subst.
   - destruct a.
-    replace ([Left t :: Gamma |= ids -| Left t :: Gamma])
-      with ([Left t.[ids] :: Gamma |= up ids -| Left t :: Gamma])
+    destruct p.
+    destruct s.
+    replace ([t :u Gamma |- ids -| t :u Gamma])
+      with ([t.[ids] :u Gamma |- up ids -| t :u Gamma])
       by autosubst.
-    apply agree_subst_L; eauto.
-    replace ([Right t :: Gamma |= ids -| Right t :: Gamma])
-      with ([Right t.[ids] :: Gamma |= up ids -| Right t :: Gamma])
+    apply agree_subst_u; eauto.
+    replace ([t :l Gamma |- ids -| t :l Gamma])
+      with ([t.[ids] :l Gamma |- up ids -| t :l Gamma])
       by autosubst.
-    apply agree_subst_R; eauto.
+    apply agree_subst_l; eauto.
     replace (ids) with (up ids) by autosubst.
-    apply agree_subst_N; eauto.
+    apply agree_subst_n; eauto.
 Qed.
 
-Lemma agree_subst_hasL Delta sigma Gamma :
-  [ Delta |= sigma -| Gamma ] ->
+Lemma agree_subst_hasU Delta sigma Gamma :
+  [ Delta |- sigma -| Gamma ] ->
   forall x A,
-    hasL Gamma x A -> 
-    [ Delta |= sigma x :- A.[sigma] -: U ].
+    hasU Gamma x A -> 
+    [ Delta |- sigma x :- A.[sigma] -: U ].
 Proof.
   induction 1; intros.
   - inv H0.
@@ -1646,12 +1505,12 @@ Proof.
         with (A.[sigma].[ren (+1)]) by autosubst.
       constructor.
       eapply agree_subst_pure; eauto.
-    + eapply eweakening_L; eauto.
+    + eapply eweakening_u; eauto.
       autosubst.
       autosubst.
   - inv H0.
   - inv H0.
-    eapply eweakening_N; eauto.
+    eapply eweakening_n; eauto.
     autosubst.
     autosubst.
   - inv H2; asimpl; eauto.
@@ -1661,7 +1520,7 @@ Proof.
   - inv H3.
   - inv H1; asimpl; eauto.
   - inv H1.
-    + assert (hasL (A :L Gamma) 0 A.[ren (+1)]).
+    + assert (hasU (A :u Gamma) 0 A.[ren (+1)]).
       constructor; eauto.
       eapply conversion.
       eapply conv_subst.
@@ -1675,16 +1534,16 @@ Proof.
   - inv H1.
 Qed.
 
-Lemma agree_subst_hasR Delta sigma Gamma :
-  [ Delta |= sigma -| Gamma ] ->
+Lemma agree_subst_hasL Delta sigma Gamma :
+  [ Delta |- sigma -| Gamma ] ->
   forall x A,
-    hasR Gamma x A -> 
-    [ Delta |= sigma x :- A.[sigma] -: L ].
+    hasL Gamma x A -> 
+    [ Delta |- sigma x :- A.[sigma] -: L ].
 Proof.
   induction 1; intros.
   - inv H0.
   - inv H0.
-    eapply eweakening_L; eauto.
+    eapply eweakening_u; eauto.
     autosubst.
     autosubst.
   - inv H0.
@@ -1695,7 +1554,7 @@ Proof.
     constructor.
     eapply agree_subst_pure; eauto.
   - inv H0.
-    eapply eweakening_N; eauto.
+    eapply eweakening_n; eauto.
     autosubst.
     autosubst.
   - inv H2; asimpl; eauto.
@@ -1708,7 +1567,7 @@ Proof.
     apply IHagree_subst.
     constructor; eauto.
   - inv H1.
-    assert (hasR (A :R Gamma) 0 A.[ren (+1)]).
+    assert (hasL (A :l Gamma) 0 A.[ren (+1)]).
     constructor; eauto.
     eapply conversion.
     apply conv_subst.
@@ -1720,8 +1579,8 @@ Proof.
 Qed.
 
 Lemma agree_subst_re_re Delta sigma Gamma :
-  [ Delta |= sigma -| Gamma ] ->
-  [ re Delta |= sigma -| re Gamma ].
+  [ Delta |- sigma -| Gamma ] ->
+  [ re Delta |- sigma -| re Gamma ].
 Proof.
   intro H.
   dependent induction H; simpl; intros; eauto.
@@ -1737,19 +1596,19 @@ Proof.
     rewrite <- H3; eauto.
   - constructor; eauto.
   - simpl in IHagree_subst.
-    eapply agree_subst_convL.
+    eapply agree_subst_convU.
     apply H.
     apply IHagree_subst.
 Qed.
 
 Lemma merge_agree_subst_inv Delta sigma Gamma :
-  [ Delta |= sigma -| Gamma ] ->
+  [ Delta |- sigma -| Gamma ] ->
   forall Gamma1 Gamma2,
     merge Gamma1 Gamma2 Gamma ->
     exists Delta1 Delta2,
       merge Delta1 Delta2 Delta /\
-      [ Delta1 |= sigma -| Gamma1 ] /\
-      [ Delta2 |= sigma -| Gamma2 ].
+      [ Delta1 |- sigma -| Gamma1 ] /\
+      [ Delta2 |- sigma -| Gamma2 ].
 Proof.
   intros H.
   dependent induction H; intros.
@@ -1760,25 +1619,25 @@ Proof.
   - inv H0.
     pose proof (IHagree_subst _ _ H4).
     first_order.
-    exists (A.[sigma] :L x).
-    exists (A.[sigma] :L x0).
+    exists (A.[sigma] :u x).
+    exists (A.[sigma] :u x0).
     repeat constructor; eauto.
   - inv H0.
     pose proof (IHagree_subst _ _ H4).
     first_order.
-    exists (A.[sigma] :R x).
-    exists (:N x0).
+    exists (A.[sigma] :l x).
+    exists (:n x0).
     repeat constructor; eauto.
   - pose proof (IHagree_subst _ _ H4).
     first_order.
-    exists (:N x).
-    exists (A.[sigma] :R x0).
+    exists (:n x).
+    exists (A.[sigma] :l x0).
     repeat constructor; eauto.
   - inv H0.
     pose proof (IHagree_subst _ _ H4).
     first_order.
-    exists (:N x).
-    exists (:N x0).
+    exists (:n x).
+    exists (:n x0).
     repeat constructor; eauto.
   - inv H2.
     pose proof (IHagree_subst _ _ H6).
@@ -1798,7 +1657,7 @@ Proof.
       exists x1.
       exists x0.
       firstorder.
-      eapply agree_subst_wkR.
+      eapply agree_subst_wkL.
       apply H.
       apply H6.
       apply H4.
@@ -1812,7 +1671,7 @@ Proof.
       exists x1.
       firstorder.
       apply agree_subst_wkN; eauto.
-      eapply agree_subst_wkR.
+      eapply agree_subst_wkL.
       apply H.
       apply H6.
       apply H5.
@@ -1824,51 +1683,51 @@ Proof.
     exists x0.
     repeat constructor; eauto.
   - inv H1.
-    assert (merge (A :L Gamma0) (A :L Gamma3) (A :L Gamma)).
+    assert (merge (A :u Gamma0) (A :u Gamma3) (A :u Gamma)).
     apply merge_left; eauto.
     specialize (IHagree_subst _ _ H1).
     first_order.
     exists x.
     exists x0.
     repeat constructor; eauto.
-    eapply agree_subst_convL; eauto.
-    eapply agree_subst_convL; eauto.
+    eapply agree_subst_convU; eauto.
+    eapply agree_subst_convU; eauto.
   - inv H1.
-    + assert (merge (A :R Gamma0) (:N Gamma3) (A :R Gamma)).
+    + assert (merge (A :l Gamma0) (:n Gamma3) (A :l Gamma)).
       constructor; eauto.
       specialize (IHagree_subst _ _ H1).
       first_order.
       exists x.
       exists x0.
       repeat constructor; eauto.
-      eapply agree_subst_convR; eauto.
-    + assert (merge (:N Gamma0) (A :R Gamma3) (A :R Gamma)).
+      eapply agree_subst_convL; eauto.
+    + assert (merge (:n Gamma0) (A :l Gamma3) (A :l Gamma)).
       constructor; eauto.
       specialize (IHagree_subst _ _ H1).
       first_order.
       exists x.
       exists x0.
       repeat constructor; eauto.
-      eapply agree_subst_convR; eauto.
+      eapply agree_subst_convL; eauto.
 Qed.
 
 Lemma substitution Gamma m A s :
-  [ Gamma |= m :- A -: s ] ->
+  [ Gamma |- m :- A -: s ] ->
   forall Delta sigma,
-    [ Delta |= sigma -| Gamma ] ->
-    [ Delta |= m.[sigma] :- A.[sigma] -: s ].
+    [ Delta |- sigma -| Gamma ] ->
+    [ Delta |- m.[sigma] :- A.[sigma] -: s ].
 Proof.
   intros H.
   dependent induction H; asimpl; intros; eauto.
   - apply axiom.
     eapply agree_subst_pure; eauto.
   - specialize (IHhas_type1 _ _ H2). asimpl in IHhas_type1.
-    pose proof (agree_subst_L A H2).
+    pose proof (agree_subst_u A H2).
     specialize (IHhas_type2 _ _ H3). asimpl in IHhas_type2.
     apply u_prod; eauto.
     eapply agree_subst_pure; eauto.
   - specialize (IHhas_type1 _ _ H2). asimpl in IHhas_type1.
-    pose proof (agree_subst_L A H2).
+    pose proof (agree_subst_u A H2).
     specialize (IHhas_type2 _ _ H3). asimpl in IHhas_type2.
     apply l_prod; eauto.
     eapply agree_subst_pure; eauto.
@@ -1880,27 +1739,27 @@ Proof.
     specialize (IHhas_type2 _ _ H2). asimpl in IHhas_type2.
     apply lolli; eauto.
     eapply agree_subst_pure; eauto.
+  - eapply agree_subst_hasU; eauto.
   - eapply agree_subst_hasL; eauto.
-  - eapply agree_subst_hasR; eauto.
   - specialize (IHhas_type1 _ _ H2). asimpl in IHhas_type1.
-    pose proof (agree_subst_L A H2).
+    pose proof (agree_subst_u A H2).
     specialize (IHhas_type2 _ _ H3).
     eapply u_lam1; eauto.
     eapply agree_subst_pure; eauto.
   - specialize (IHhas_type1 _ _ H2). asimpl in IHhas_type1.
-    pose proof (agree_subst_R A H2).
+    pose proof (agree_subst_l A H2).
     specialize (IHhas_type2 _ _ H3). asimpl in IHhas_type2.
     eapply u_lam2; eauto.
     eapply agree_subst_pure; eauto.
     asimpl; eauto.
   - pose proof (agree_subst_re_re H1).
     specialize (IHhas_type1 _ _ H2). asimpl in IHhas_type1.
-    pose proof (agree_subst_L A H1).
+    pose proof (agree_subst_u A H1).
     specialize (IHhas_type2 _ _ H3).
     eapply l_lam1; eauto.
   - pose proof (agree_subst_re_re H1).
     specialize (IHhas_type1 _ _ H2). asimpl in IHhas_type1.
-    pose proof (agree_subst_R A H1).
+    pose proof (agree_subst_l A H1).
     specialize (IHhas_type2 _ _ H3). asimpl in IHhas_type2.
     eapply l_lam2; eauto.
     asimpl; eauto.
@@ -1922,13 +1781,13 @@ Proof.
     apply IHhas_type; eauto.
 Qed.
 
-Lemma substitutionL Gamma1 m A B s :
-  [ A :L Gamma1 |= m :- B -: s ] ->
+Lemma substitutionU Gamma1 m A B s :
+  [ A :u Gamma1 |- m :- B -: s ] ->
   forall Gamma2 Gamma n,
     value n ->
     merge Gamma1 Gamma2 Gamma -> 
-    [ Gamma2 |= n :- A -: U ] -> 
-    [ Gamma |= m.[n/] :- B.[n/] -: s ].
+    [ Gamma2 |- n :- A -: U ] -> 
+    [ Gamma |- m.[n/] :- B.[n/] -: s ].
 Proof.
   intros.
   eapply substitution.
@@ -1936,7 +1795,7 @@ Proof.
   pose proof (value_sound H2 H0).
   pose proof (merge_pure2 H1 H3).
   rewrite H4.
-  apply agree_subst_wkL; eauto.
+  apply agree_subst_wkU; eauto.
   apply agree_subst_refl.
   pose proof (merge_re_re H1).
   destruct H5.
@@ -1947,11 +1806,11 @@ Proof.
 Qed.
 
 Lemma substitutionN Gamma1 m A B s :
-  [ :N Gamma1 |= m :- B -: s ] ->
+  [ :n Gamma1 |- m :- B -: s ] ->
   forall Gamma2 n t,
     value n ->
-    [ Gamma2 |= n :- A -: t ] -> 
-    [ Gamma1 |= m.[n/] :- B.[n/] -: s ].
+    [ Gamma2 |- n :- A -: t ] -> 
+    [ Gamma1 |- m.[n/] :- B.[n/] -: s ].
 Proof.
   intros.
   eapply substitution.
@@ -1960,28 +1819,42 @@ Proof.
   apply agree_subst_refl.
 Qed.
 
-Lemma substitutionR Gamma1 m A B s :
-  [ A :R Gamma1 |= m :- B -: s ] ->
+Lemma substitutionL Gamma1 m A B s :
+  [ A :l Gamma1 |- m :- B -: s ] ->
   forall Gamma2 Gamma n,
     value n ->
     merge Gamma1 Gamma2 Gamma -> 
-    [ Gamma2 |= n :- A -: L ] -> 
-    [ Gamma |= m.[n/] :- B.[n/] -: s ].
+    [ Gamma2 |- n :- A -: L ] -> 
+    [ Gamma |- m.[n/] :- B.[n/] -: s ].
 Proof.
   intros.
   eapply substitution.
   apply H.
-  eapply agree_subst_wkR; asimpl; eauto.
+  eapply agree_subst_wkL; asimpl; eauto.
+  apply agree_subst_refl.
+Qed.
+
+Lemma context_convU Gamma m A B C s :
+  B === A -> 
+  [ A :u Gamma |- m :- C -: s ] -> 
+  [ B :u Gamma |- m :- C -: s ].
+Proof.
+  move=> conv tp. 
+  cut ([ B :u Gamma |- m.[ids] :- C.[ids] -: s ]). autosubst.
+  eapply substitution.
+  apply tp.
+  eapply agree_subst_convU; simpl.
+  apply conv.
   apply agree_subst_refl.
 Qed.
 
 Lemma context_convL Gamma m A B C s :
   B === A -> 
-  [ A :L Gamma |= m :- C -: s ] -> 
-  [ B :L Gamma |= m :- C -: s ].
+  [ A :l Gamma |- m :- C -: s ] -> 
+  [ B :l Gamma |- m :- C -: s ].
 Proof.
   move=> conv tp. 
-  cut ([ B :L Gamma |= m.[ids] :- C.[ids] -: s ]). autosubst.
+  cut ([ B :l Gamma |- m.[ids] :- C.[ids] -: s ]). autosubst.
   eapply substitution.
   apply tp.
   eapply agree_subst_convL; simpl.
@@ -1989,23 +1862,8 @@ Proof.
   apply agree_subst_refl.
 Qed.
 
-Lemma context_convR Gamma m A B C s :
-  B === A -> 
-  [ A :R Gamma |= m :- C -: s ] -> 
-  [ B :R Gamma |= m :- C -: s ].
-Proof.
-  move=> conv tp. 
-  cut ([ B :R Gamma |= m.[ids] :- C.[ids] -: s ]). autosubst.
-  eapply substitution.
-  apply tp.
-  eapply agree_subst_convR; simpl.
-  apply conv.
-  apply agree_subst_refl.
-Qed.
-
-Lemma sort_inj s1 s2 l1 l2 :
-  Sort s1 l1 === Sort s2 l2 ->
-  s1 = s2 /\ l1 = l2.
+Lemma sort_inj s1 s2 :
+  Sort s1 === Sort s2 -> s1 = s2.
 Proof.
   intros.
   apply church_rosser in H.
@@ -2075,104 +1933,42 @@ Proof.
   inv H2; eauto.
 Qed.
 
-Lemma tyProd_invX Gamma A B s srt :
-  [ re Gamma |= TyProd A B s :- srt -: U ] -> 
-  forall l, srt === Sort U l ->
-    [ re Gamma |= A :- Sort U l -: U ] /\ 
-    [ A :L re Gamma |= B :- Sort s l -: U ].
+Lemma tyProd_inv Gamma A B s :
+  [ re Gamma |- TyProd A B s :- Sort U -: U ] -> 
+  [ re Gamma |- A :- Sort U -: U ] /\ [ A :u re Gamma |- B :- Sort s -: U ].
 Proof.
-  move e:(TyProd A B s) => n tp. 
-  elim: tp A B s e => //{Gamma n}.
-  move=> Gamma A B s l p tp1 _ tp2 _ A0 B0 s0 [->->->] l0 /sort_inj[_<-] => //.
-  move=> Gamma A B m s e1 tp1 ih A0 B0 s0 h l e2.
-  eapply ih; eauto.
-  eapply conv_trans.
-  apply e1.
-  apply e2.
+  move e:(TyProd A B s) => n tp. elim: tp A B s e => //{Gamma n}.
+  move=> Gamma A B s p tp1 _ tp2 _ A0 B0 s0 [->->->] => //.
 Qed.
 
-Lemma tyProd_inv Gamma A B s l :
-  [ re Gamma |= TyProd A B s :- Sort U l -: U ] -> 
-  [ re Gamma |= A :- Sort U l -: U ] /\ 
-  [ A :L re Gamma |= B :- Sort s l -: U ].
+Lemma arrow_inv Gamma A B s :
+  [ re Gamma |- Arrow A B s :- Sort U -: U ] ->
+  [ re Gamma |- A :- Sort L -: U ] /\ [ re Gamma |- B :- Sort s -: U ].
 Proof.
-  intros.
-  eapply tyProd_invX; eauto.
+  move e:(Arrow A B s) => n tp. elim: tp A B s e => //{Gamma n}.
+  move=> Gamma A B s p tp1 _ tp2 _ A0 B0 s0 [->->->] => //.
 Qed.
 
-Lemma arrow_invX Gamma A B s srt :
-  [ re Gamma |= Arrow A B s :- srt -: U ] ->
-  forall l, srt === Sort U l ->
-    [ re Gamma |= A :- Sort L l -: U ] /\ 
-    [ re Gamma |= B :- Sort s l -: U ].
+Lemma lnProd_inv Gamma A B s :
+  [ re Gamma |- LnProd A B s :- Sort L -: U ] ->
+  [ re Gamma |- A :- Sort U -: U ] /\ [ A :u re Gamma |- B :- Sort s -: U ].
 Proof.
-  move e:(Arrow A B s) => n tp. 
-  elim: tp A B s e => //{Gamma n}.
-  move=> Gamma A B s l p tp1 _ tp2 _ A0 B0 s0 [->->->] l0 /sort_inj[_<-] => //.
-  move=> Gamma A B m s e1 tp1 ih A0 B0 s0 h l e2.
-  eapply ih; eauto.
-  eapply conv_trans.
-  apply e1.
-  apply e2.
+  move e:(LnProd A B s) => n tp. elim: tp A B s e => //{Gamma n}.
+  move=> Gamma A B s p tp1 _ tp2 _ A0 B0 s0 [->->->] => //.
 Qed.
 
-Lemma arrow_inv Gamma A B s l :
-  [ re Gamma |= Arrow A B s :- Sort U l -: U ] ->
-  [ re Gamma |= A :- Sort L l -: U ] /\ 
-  [ re Gamma |= B :- Sort s l -: U ].
+Lemma lolli_inv Gamma A B s :
+  [ re Gamma |- Lolli A B s :- Sort L -: U ] ->
+  [ re Gamma |- A :- Sort L -: U ] /\ [ re Gamma |- B :- Sort s -: U ].
 Proof.
-  intros.
-  eapply arrow_invX; eauto.
-Qed.
-
-Lemma lnProd_invX Gamma A B s srt :
-  [ re Gamma |= LnProd A B s :- srt -: U ] ->
-  forall l, srt === Sort L l ->
-    [ re Gamma |= A :- Sort U l -: U ] /\ 
-    [ A :L re Gamma |= B :- Sort s l -: U ].
-Proof.
-  move e:(LnProd A B s) => n tp. 
-  elim: tp A B s e => //{Gamma n}.
-  move=> Gamma A B s l p tp1 _ tp2 _ A0 B0 s0 [->->->] l0 /sort_inj[_<-] => //.
-  move=> Gamma A B m s e1 tp1 ih A0 B0 s0 h l e2.
-  eapply ih; eauto.
-  eapply conv_trans.
-  apply e1.
-  apply e2.
-Qed.
-
-Lemma lnProd_inv Gamma A B s l :
-  [ re Gamma |= LnProd A B s :- Sort L l -: U ] ->
-  [ re Gamma |= A :- Sort U l -: U ] /\ 
-  [ A :L re Gamma |= B :- Sort s l -: U ].
-Proof.
-  intros.
-  eapply lnProd_invX; eauto.
-Qed.
-
-Lemma lolli_invX Gamma A B s srt :
-  [ re Gamma |= Lolli A B s :- srt -: U ] ->
-  forall l, srt === Sort L l ->
-    [ re Gamma |= A :- Sort L l -: U ] /\ 
-    [ re Gamma |= B :- Sort s l -: U ].
-Proof.
-  move e:(Lolli A B s) => n tp. 
-  elim: tp A B s e => //{Gamma n}.
-  move=> Gamma A B s l p tp1 _ tp2 _ A0 B0 s0 [->->->] l0 /sort_inj[_<-] => //.
-  move=> Gamma A B m s e1 tp1 ih A0 B0 s0 h l e2.
-  eapply ih; eauto.
-  eapply conv_trans.
-  apply e1.
-  apply e2.
-Qed.
-
-Lemma lolli_inv Gamma A B s l :
-  [ re Gamma |= Lolli A B s :- Sort L l -: U ] ->
-  [ re Gamma |= A :- Sort L l -: U ] /\ 
-  [ re Gamma |= B :- Sort s l -: U ].
-Proof.
-  intros.
-  eapply lolli_invX; eauto.
+  move e:(Lolli A B s) => n tp. elim: tp A B s e => //{Gamma n}.
+  move=> Gamma A B s p tp1 _ tp2 _ A0 B0 s0 [->->->] => //.
+  move=> Gamma A B m s p tp ih A0 B0 s0 e.
+  apply ih in e.
+  first_order; eauto.
+  eapply conversion.
+  apply p.
+  apply H.
 Qed.
 
 Ltac red_inv m H :=
@@ -2210,10 +2006,10 @@ Ltac solve_conv :=
   end; eauto.
 
 Lemma u_lam1_inv Gamma n C :
-  [ Gamma |= Lam n :- C -: U ] -> 
+  [ Gamma |- Lam n :- C -: U ] -> 
   forall A B s, 
     (C === TyProd A B s) ->
-    [ A :L Gamma |= n :- B -: s ].
+    [ A :u Gamma |- n :- B -: s ].
 Proof.
   intros.
   dependent induction H.
@@ -2221,10 +2017,10 @@ Proof.
     first_order.
     eapply conversion.
     apply H3.
-    eapply context_convL.
+    eapply context_convU.
     apply conv_sym; apply H2.
     rewrite <- H4; eauto.
-  + solve_conv; exfalso; eauto.
+  + exfalso; solve_conv.
   + apply IHhas_type; eauto.
     eapply conv_trans.
     apply H.
@@ -2232,21 +2028,21 @@ Proof.
 Qed.
 
 Lemma u_lam2_inv Gamma n C :
-  [ Gamma |= Lam n :- C -: U ] -> 
+  [ Gamma |- Lam n :- C -: U ] -> 
   forall A B s, 
     (C === Arrow A B s) ->
-    [ A :R Gamma |= n :- B.[ren (+1)] -: s ].
+    [ A :l Gamma |- n :- B.[ren (+1)] -: s ].
 Proof.
   intros.
   dependent induction H.
-  + solve_conv; exfalso; eauto.
+  + exfalso; solve_conv.
   + apply arrow_inj in H2.
     first_order.
     eapply conversion.
     apply conv_subst.
     apply ren_v_subst.
     apply H3.
-    eapply context_convR.
+    eapply context_convL.
     apply conv_sym; apply H2.
     rewrite <- H4; eauto.
   + apply IHhas_type; eauto.
@@ -2256,10 +2052,10 @@ Proof.
 Qed.
 
 Lemma l_lam1_inv Gamma n C :
-  [ Gamma |= Lam n :- C -: L ] -> 
+  [ Gamma |- Lam n :- C -: L ] -> 
   forall A B s, 
     (C === LnProd A B s) ->
-    [ A :L Gamma |= n :- B -: s ].
+    [ A :u Gamma |- n :- B -: s ].
 Proof.
   intros.
   dependent induction H.
@@ -2267,7 +2063,7 @@ Proof.
     first_order.
     eapply conversion.
     apply H2.
-    eapply context_convL.
+    eapply context_convU.
     apply conv_sym; apply H1.
     rewrite <- H3; eauto.
   + solve_conv; exfalso; eauto.
@@ -2278,21 +2074,21 @@ Proof.
 Qed.
 
 Lemma l_lam2_inv Gamma n C :
-  [ Gamma |= Lam n :- C -: L ] -> 
+  [ Gamma |- Lam n :- C -: L ] -> 
   forall A B s, 
     (C === Lolli A B s) ->
-    [ A :R Gamma |= n :- B.[ren (+1)] -: s ].
+    [ A :l Gamma |- n :- B.[ren (+1)] -: s ].
 Proof.
   intros.
   dependent induction H.
-  + solve_conv; exfalso; eauto.
+  + exfalso; solve_conv.
   + apply lolli_inj in H1.
     first_order.
     eapply conversion.
     apply conv_subst.
     apply ren_v_subst.
     apply H2.
-    eapply context_convR.
+    eapply context_convL.
     apply conv_sym; apply H1.
     rewrite <- H3; eauto.
   + apply IHhas_type; eauto.
@@ -2302,9 +2098,9 @@ Proof.
 Qed.
 
 Theorem preservation Gamma m A s :
-  [ Gamma |= m :- A -: s ] ->
+  [ Gamma |- m :- A -: s ] ->
   forall n, pstep m n -> 
-    [ Gamma |= n :- A -: s ].
+    [ Gamma |- n :- A -: s ].
 Proof.
   intros.
   dependent induction H.
@@ -2314,14 +2110,14 @@ Proof.
     specialize (IHhas_type1 _ H7).
     specialize (IHhas_type2 _ H8).
     apply u_prod; eauto.
-    eapply context_convL.
+    eapply context_convU.
     eapply conv1i; eauto.
     apply IHhas_type2.
   - inv H2.
     specialize (IHhas_type1 _ H7).
     specialize (IHhas_type2 _ H8).
     apply l_prod; eauto.
-    eapply context_convL.
+    eapply context_convU.
     eapply conv1i; eauto.
     apply IHhas_type2.
   - inv H2.
@@ -2367,7 +2163,7 @@ Proof.
       apply pstep_refl.
       eapply conversion.
       apply conv1i; eauto.
-      eapply substitutionL.
+      eapply substitutionU.
       apply IHhas_type1.
       eapply pstep_value; eauto.
       apply H1.
@@ -2382,7 +2178,7 @@ Proof.
       specialize (IHhas_type2 _ H8).
       eapply u_lam2_inv in IHhas_type1; eauto.
       replace B with (B.[ren (+1)].[v'/]) by autosubst.
-      eapply substitutionR.
+      eapply substitutionL.
       apply IHhas_type1.
       eapply pstep_value; eauto.
       apply H1.
@@ -2406,7 +2202,7 @@ Proof.
       apply pstep_refl.
       eapply conversion.
       apply conv1i; eauto.
-      eapply substitutionL.
+      eapply substitutionU.
       apply IHhas_type1.
       eapply pstep_value; eauto.
       apply H1.
@@ -2421,7 +2217,7 @@ Proof.
       specialize (IHhas_type2 _ H8).
       eapply l_lam2_inv in IHhas_type1; eauto.
       replace B with (B.[ren (+1)].[v'/]) by autosubst.
-      eapply substitutionR.
+      eapply substitutionL.
       apply IHhas_type1.
       eapply pstep_value; eauto.
       apply H1.
@@ -2432,8 +2228,8 @@ Qed.
 Corollary preservation_step m n :
   step m n ->
   forall Gamma A s,
-    [ Gamma |= m :- A -: s ] ->
-    [ Gamma |= n :- A -: s ].
+    [ Gamma |- m :- A -: s ] ->
+    [ Gamma |- n :- A -: s ].
 Proof.
   intros.
   eapply preservation.
@@ -2444,8 +2240,8 @@ Qed.
 Corollary preservation_star_step m n :
   star step m n ->
   forall Gamma A s,
-    [ Gamma |= m :- A -: s ] ->
-    [ Gamma |= n :- A -: s ].
+    [ Gamma |- m :- A -: s ] ->
+    [ Gamma |- n :- A -: s ].
 Proof.
   intro H.
   dependent induction H; intros; eauto.
@@ -2455,20 +2251,20 @@ Proof.
 Qed.
 
 Lemma canonical_tyProd m C :
-  [ nil |= m :- C -: U ] -> value m ->
+  [ nil |- m :- C -: U ] -> value m ->
   forall A B s, 
     C === TyProd A B s -> exists m', m = Lam m'.
 Proof.
   intros.
   dependent induction H.
-  - solve_conv; exfalso; eauto.
-  - solve_conv; exfalso; eauto.
-  - solve_conv; exfalso; eauto.
-  - solve_conv; exfalso; eauto.
-  - solve_conv; exfalso; eauto.
+  - exfalso; solve_conv.
+  - exfalso; solve_conv.
+  - exfalso; solve_conv.
+  - exfalso; solve_conv.
+  - exfalso; solve_conv.
   - inv H.
   - exists n; eauto.
-  - solve_conv; exfalso; eauto.
+  - exfalso; solve_conv.
   - inv H2.
   - inv H2.
   - inv H2.
@@ -2480,7 +2276,7 @@ Proof.
 Qed.
 
 Lemma canonical_lnProd m C :
-  [ nil |= m :- C -: L ] -> value m ->
+  [ nil |- m :- C -: L ] -> value m ->
   forall A B s, 
     C === LnProd A B s -> exists m', m = Lam m'.
 Proof.
@@ -2488,7 +2284,7 @@ Proof.
   dependent induction H.
   - inv H.
   - exists n; eauto.
-  - solve_conv; exfalso; eauto.
+  - exfalso; solve_conv.
   - inv H2.
   - inv H2.
   - inv H2.
@@ -2500,19 +2296,19 @@ Proof.
 Qed.
 
 Lemma canonical_arrow m C :
-  [ nil |= m :- C -: U ] -> value m ->
+  [ nil |- m :- C -: U ] -> value m ->
   forall A B s, 
     C === Arrow A B s -> exists m', m = Lam m'.
 Proof.
   intros.
   dependent induction H.
-  - solve_conv; exfalso; eauto.
-  - solve_conv; exfalso; eauto.
-  - solve_conv; exfalso; eauto.
-  - solve_conv; exfalso; eauto.
-  - solve_conv; exfalso; eauto.
+  - exfalso; solve_conv.
+  - exfalso; solve_conv.
+  - exfalso; solve_conv.
+  - exfalso; solve_conv.
+  - exfalso; solve_conv.
   - inv H.
-  - solve_conv; exfalso; eauto.
+  - exfalso; solve_conv.
   - exists n; eauto.
   - inv H2.
   - inv H2.
@@ -2525,14 +2321,14 @@ Proof.
 Qed.
 
 Lemma canonical_lolli m C :
-  [ nil |= m :- C -: L ] -> value m ->
+  [ nil |- m :- C -: L ] -> value m ->
   forall A B s, 
     C === Lolli A B s -> exists m', m = Lam m'.
 Proof.
   intros.
   dependent induction H.
   - inv H.
-  - solve_conv; exfalso; eauto.
+  - exfalso; solve_conv.
   - exists n; eauto.
   - inv H2.
   - inv H2.
@@ -2545,7 +2341,7 @@ Proof.
 Qed.
 
 Theorem progress m A s :
-  [ nil |= m :- A -: s ] -> value m \/ exists n, step m n.
+  [ nil |- m :- A -: s ] -> value m \/ exists n, step m n.
 Proof.
   intros.
   dependent induction H.
